vSet: change prime notation

theories/νSet/νSet.v
@@ -19,7 +19,7 @@ Variable arity: HSet.
 Fixpoint mkFrameTypes p: Type :=
   match p with
   | 0 => unit
-  | S p => { frames'': mkFrameTypes p &T HSet }
+  | S p => { frames: mkFrameTypes p &T HSet }
   end.
 
 (** The type of lists [painting(p+n,0);...;painting(p+n,p-1)] for arbitrary n *)
@@ -27,8 +27,8 @@ Fixpoint mkFrameTypes p: Type :=
 Fixpoint mkPaintingTypes p: mkFrameTypes p -> Type :=
   match p with
   | 0 => fun _ => unit
-  | S p => fun frames'' =>
-    { painting'': mkPaintingTypes p frames''.1 &T frames''.2 -> HSet }
+  | S p => fun frames =>
+    { paintings: mkPaintingTypes p frames.1 &T frames.2 -> HSet }
   end.
 
 Class RestrFrameTypeBlock p := {
@@ -63,84 +63,84 @@ That is, we build:
 *)
 
 Definition mkRestrFrameTypesStep {p n}
-  (frames'': mkFrameTypes p.+1)
+  (frames: mkFrameTypes p.+1)
   (prev: RestrFrameTypeBlock p) :=
   { R: prev.(RestrFrameTypesDef) &T
-    forall q (Hq: q <= n) (ε: arity), (prev.(FrameDef) R).2 -> frames''.2 }.
+    forall q (Hq: q <= n) (ε: arity), (prev.(FrameDef) R).2 -> frames.2 }.
 
 Definition mkLayer {p n}
-  {frames'': mkFrameTypes p.+1}
-  {paintings'': mkPaintingTypes p.+1 frames''}
+  {frames: mkFrameTypes p.+1}
+  {paintings: mkPaintingTypes p.+1 frames}
   {prev: RestrFrameTypeBlock p}
-  (restrFrames: mkRestrFrameTypesStep (n := n) frames'' prev)
+  (restrFrames: mkRestrFrameTypesStep (n := n) frames prev)
   (d: (prev.(FrameDef) restrFrames.1).2) :=
-  hforall ε, paintings''.2 (restrFrames.2 0 leY_O ε d).
+  hforall ε, paintings.2 (restrFrames.2 0 leY_O ε d).
 
-Fixpoint mkRestrFrameTypesAndFrames' {p n}: forall (frames'': mkFrameTypes p)
-  (paintings'': mkPaintingTypes p frames''), RestrFrameTypeBlock p :=
+Fixpoint mkRestrFrameTypesAndFrames {p n}: forall (frames: mkFrameTypes p)
+  (paintings: mkPaintingTypes p frames), RestrFrameTypeBlock p :=
   match p with
-  | 0 => fun frames'' paintings'' =>
+  | 0 => fun frames paintings =>
     {|
       RestrFrameTypesDef := unit;
       FrameDef _ := (tt; hunit): mkFrameTypes 1
     |}
-  | p.+1 => fun frames'' paintings'' =>
+  | p.+1 => fun frames paintings =>
     let prev :=
-      mkRestrFrameTypesAndFrames' (n := n.+1) frames''.1 paintings''.1 in
+      mkRestrFrameTypesAndFrames (n := n.+1) frames.1 paintings.1 in
     let frames' := prev.(FrameDef) in
     {|
-      RestrFrameTypesDef := mkRestrFrameTypesStep (n := n) frames'' prev;
+      RestrFrameTypesDef := mkRestrFrameTypesStep (n := n) frames prev;
       FrameDef R :=
         (frames' R.1; { d: (frames' R.1).2 &
-          mkLayer (paintings'' := paintings'') R d }): mkFrameTypes p.+2
+          mkLayer (paintings := paintings) R d }): mkFrameTypes p.+2
     |}
   end.
 
 Class DepsRestr p n := {
-  _frames'': mkFrameTypes p;
-  _paintings'': mkPaintingTypes p _frames'';
-  _restrFrames': (mkRestrFrameTypesAndFrames' _frames'' _paintings''
+  _frames: mkFrameTypes p;
+  _paintings: mkPaintingTypes p _frames;
+  _restrFrames: (mkRestrFrameTypesAndFrames _frames _paintings
     (n := n)).(RestrFrameTypesDef);
 }.
 
 Generalizable Variables p n.
 
-Definition mkFrames' `(deps: DepsRestr p n): mkFrameTypes p.+1 :=
-  (mkRestrFrameTypesAndFrames' deps.(_frames'')
-    deps.(_paintings'')).(FrameDef) deps.(_restrFrames').
+Definition mkFrames `(deps: DepsRestr p n): mkFrameTypes p.+1 :=
+  (mkRestrFrameTypesAndFrames deps.(_frames)
+    deps.(_paintings)).(FrameDef) deps.(_restrFrames).
 
-Definition mkFrame' `(deps: DepsRestr p n): HSet := (mkFrames' deps).2.
+Definition mkFrame `(deps: DepsRestr p n): HSet := (mkFrames deps).2.
 
 Class DepRestr `(deps: DepsRestr p n.+1) := {
-  _frame'': HSet;
-  _painting'': _frame'' -> HSet;
-  _restrFrame': forall q {Hq: q <= n} (ε: arity),
-    mkFrame' (n := n.+1) deps -> _frame'';
+  _frame: HSet;
+  _painting: _frame -> HSet;
+  _restrFrame: forall q {Hq: q <= n} (ε: arity),
+    mkFrame (n := n.+1) deps -> _frame;
 }.
 
 #[local]
 Instance consDep `(deps: DepsRestr p n.+1)
   (dep: DepRestr deps): DepsRestr p.+1 n :=
 {|
-  _frames'' := (deps.(_frames''); dep.(_frame'')): mkFrameTypes p.+1;
-  _paintings'' := (deps.(_paintings''); dep.(_painting''));
-  _restrFrames' := (deps.(_restrFrames'); dep.(_restrFrame'));
+  _frames := (deps.(_frames); dep.(_frame)): mkFrameTypes p.+1;
+  _paintings := (deps.(_paintings); dep.(_painting));
+  _restrFrames := (deps.(_restrFrames); dep.(_restrFrame));
 |}.
 
 #[local]
 Instance proj1Deps `(deps: DepsRestr p.+1 n): DepsRestr p n.+1 :=
 {|
-  _frames'' := deps.(_frames'').1;
-  _paintings'' := deps.(_paintings'').1;
-  _restrFrames' := deps.(_restrFrames').1;
+  _frames := deps.(_frames).1;
+  _paintings := deps.(_paintings).1;
+  _restrFrames := deps.(_restrFrames).1;
 |}.
 
 #[local]
 Instance proj2Deps `(deps: DepsRestr p.+1 n): DepRestr (proj1Deps deps) :=
 {|
-  _frame'' := deps.(_frames'').2;
-  _painting'' := deps.(_paintings'').2;
-  _restrFrame' := deps.(_restrFrames').2;
+  _frame := deps.(_frames).2;
+  _painting := deps.(_paintings).2;
+  _restrFrame := deps.(_restrFrames).2;
 |}.
 
 Declare Scope depsrestr_scope.
@@ -155,7 +155,7 @@ Notation "( x ; y )" := (consDep x%_depsrestr y)
 
 Inductive DepsRestrExtension {p}: forall {n}, DepsRestr p n -> Type :=
 | TopDep {deps}:
-  forall E': mkFrame' deps -> HSet, DepsRestrExtension (n := 0) deps
+  forall E': mkFrame deps -> HSet, DepsRestrExtension (n := 0) deps
 | AddDep {n deps} dep:
   DepsRestrExtension (consDep deps dep) -> DepsRestrExtension (n := n.+1) deps.
 
@@ -167,26 +167,26 @@ Notation "( x ; y )" := (AddDep x y)
 
 (* Example: if p := 0, extraDeps := ([],E') mkPainting:= [E'] *)
 
-Fixpoint mkPainting' `{deps: DepsRestr p n}
+Fixpoint mkPainting `{deps: DepsRestr p n}
   (extraDeps: DepsRestrExtension deps):
-  mkFrame' deps -> HSet :=
+  mkFrame deps -> HSet :=
   match extraDeps with
-  | @TopDep _ deps E' => fun (d: mkFrame' deps) => E' d
-  | @AddDep _ _ deps dep extraDeps => fun (d: mkFrame' deps) =>
-      {l: mkLayer (deps; dep).(_restrFrames') d & mkPainting' extraDeps (d; l)}
+  | @TopDep _ deps E' => fun (d: mkFrame deps) => E' d
+  | @AddDep _ _ deps dep extraDeps => fun (d: mkFrame deps) =>
+      {l: mkLayer (deps; dep).(_restrFrames) d & mkPainting extraDeps (d; l)}
   end.
 
-Fixpoint mkPaintings' {p n}: forall `{deps: DepsRestr p n}
-  (extraDeps: DepsRestrExtension deps), mkPaintingTypes p.+1 (mkFrames' deps) :=
+Fixpoint mkPaintings {p n}: forall `{deps: DepsRestr p n}
+  (extraDeps: DepsRestrExtension deps), mkPaintingTypes p.+1 (mkFrames deps) :=
   match p with
-  | 0 => fun deps extraDeps => (tt; mkPainting' extraDeps)
+  | 0 => fun deps extraDeps => (tt; mkPainting extraDeps)
   | S p => fun deps extraDeps =>
-    (mkPaintings' (deps.(2); extraDeps)%extradeps; mkPainting' extraDeps)
+    (mkPaintings (deps.(2); extraDeps)%extradeps; mkPainting extraDeps)
   end.
 
 Lemma unfoldPaintingProj `{deps: DepsRestr p n}
-  {extraDeps: DepsRestrExtension deps} {d: mkFrame' deps}:
-   mkPainting' extraDeps d = (mkPaintings' extraDeps).2 d.
+  {extraDeps: DepsRestrExtension deps} {d: mkFrame deps}:
+   mkPainting extraDeps d = (mkPaintings extraDeps).2 d.
 Proof.
   now destruct p.
 Defined.
@@ -208,18 +208,10 @@ Defined.
 
 Definition mkRestrFrameTypes `{deps: DepsRestr p n}
   (extraDeps: DepsRestrExtension deps) :=
-  (mkRestrFrameTypesAndFrames' (n := n) (mkFrames' deps)
-    (mkPaintings' extraDeps)).(RestrFrameTypesDef).
+  (mkRestrFrameTypesAndFrames (n := n) (mkFrames deps)
+    (mkPaintings extraDeps)).(RestrFrameTypesDef).
 
-(* Same, but restricted to p-1, that is, the types of:
-    [restrFrame(p+1+n,0);...;restrFrame(p+1+n,p-1)] *)
-
-Definition mkPrevRestrFrameTypes `(deps: DepsRestr p n)
-  (extraDeps: DepsRestrExtension deps) :=
-  (mkRestrFrameTypesAndFrames' (n := n.+1) (mkFrames' deps).1
-    (mkPaintings' extraDeps).1).(RestrFrameTypesDef).
-
-(** We combining mkFrames', mkPaintings' and an assumed restrFrames.
+(** We combining mkFrames, mkPaintings and an assumed restrFrames.
      That is, from:
        [frame(p-1+n,0);...;frame(p-1+n,p-1)]
        [painting(p-1+n,0);...;painting(p-1+n,p-1)]
@@ -240,26 +232,10 @@ Definition mkDepsRestr `{deps: DepsRestr p n}
   {extraDeps: DepsRestrExtension deps}
   (restrFrames: mkRestrFrameTypes extraDeps) :=
 {|
-  _frames'' := mkFrames' deps;
-  _paintings'' := mkPaintings' extraDeps;
-  _restrFrames' := restrFrames;
+  _frames := mkFrames deps;
+  _paintings := mkPaintings extraDeps;
+  _restrFrames := restrFrames;
 |}.
-
-(** Thus being able to build frame(p+1+n,p+1) from the same assumptions *)
-
-Definition mkFrame `{deps: DepsRestr p n} {extraDeps: DepsRestrExtension deps}
-  (restrFrames: mkRestrFrameTypes extraDeps) :=
-  mkFrame' (mkDepsRestr restrFrames).
-
-(** By restriction, we can thus build frame(p+1+n,p). Note that mkPrevFrame
-    could not be built by calling mkFrame' on p and n+1 (rather than on
-    p+1 and n, then restricting) because it would require knowing deps for
-    p and n+1 instead of only p and n *)
-
-Definition mkPrevFrame `{deps: DepsRestr p n}
-  {extraDeps: DepsRestrExtension deps}
-  (restrFrames: mkRestrFrameTypes extraDeps) :=
-  mkFrame' (mkDepsRestr restrFrames).(1).
 
 Class CohFrameTypeBlock `{deps: DepsRestr p n}
   {extraDeps: DepsRestrExtension deps} := {
@@ -267,44 +243,44 @@ Class CohFrameTypeBlock `{deps: DepsRestr p n}
   RestrFramesDef: CohFrameTypesDef -> mkRestrFrameTypes extraDeps
 }.
 
-Definition RestrPaintingType' `{deps: DepsRestr p n.+1} (dep: DepRestr deps)
+Definition RestrPaintingType `{deps: DepsRestr p n.+1} (dep: DepRestr deps)
   (extraDeps: DepsRestrExtension (deps; dep)) :=
-  forall q (Hq: q <= n) ε (d: mkFrame' deps),
-  (mkPaintings' (dep; extraDeps)).2 d ->
-  dep.(_painting'') (dep.(_restrFrame') q ε d).
+  forall q (Hq: q <= n) ε (d: mkFrame deps),
+  (mkPaintings (dep; extraDeps)).2 d ->
+  dep.(_painting) (dep.(_restrFrame) q ε d).
 
-Fixpoint RestrPaintingTypes' {p}: forall `{deps: DepsRestr p n}
+Fixpoint RestrPaintingTypes {p}: forall `{deps: DepsRestr p n}
   (extraDeps: DepsRestrExtension deps), Type :=
   match p with
   | 0 => fun _ _ _ => unit
   | S p =>
     fun n deps extraDeps =>
-    { _: RestrPaintingTypes' (deps.(2); extraDeps) &T
-      RestrPaintingType' deps.(2) extraDeps }
+    { _: RestrPaintingTypes (deps.(2); extraDeps) &T
+      RestrPaintingType deps.(2) extraDeps }
   end.
 
 Definition mkCohFrameTypesStep `{deps: DepsRestr p.+1 n}
   {extraDeps: DepsRestrExtension deps}
-  {restrPaintings': RestrPaintingTypes' extraDeps}
+  {restrPaintings: RestrPaintingTypes extraDeps}
   (prev: CohFrameTypeBlock (extraDeps := (deps.(2); extraDeps))): Type :=
   { Q: prev.(CohFrameTypesDef) &T
     forall r q (Hrq: r <= q) (Hq: q <= n) (ε ω: arity) d,
-    deps.(_restrFrames').2 q Hq ε
+    deps.(_restrFrames).2 q Hq ε
       ((prev.(RestrFramesDef) Q).2 r (Hrq ↕ (↑ Hq)) ω d) =
-    deps.(_restrFrames').2 r (Hrq ↕ Hq) ω
+    deps.(_restrFrames).2 r (Hrq ↕ Hq) ω
       ((prev.(RestrFramesDef) Q).2 q.+1 (⇑ Hq) ε d) }.
 
 Definition mkRestrLayer `{deps: DepsRestr p.+1 n}
   {extraDeps: DepsRestrExtension deps}
-  (restrPaintings': RestrPaintingTypes' extraDeps)
+  (restrPaintings: RestrPaintingTypes extraDeps)
   {prev: CohFrameTypeBlock (extraDeps := (deps.(2); extraDeps))}
-  (cohFrames: mkCohFrameTypesStep (restrPaintings' := restrPaintings') prev)
+  (cohFrames: mkCohFrameTypesStep (restrPaintings := restrPaintings) prev)
   q (Hq: q <= n) (ε: arity)
-  (d: mkPrevFrame (prev.(RestrFramesDef) cohFrames.1)):
-  mkLayer (prev.(RestrFramesDef) cohFrames.1) d -> mkLayer deps.(_restrFrames')
+  (d: mkFrame (mkDepsRestr (prev.(RestrFramesDef) cohFrames.1)).(1)):
+  mkLayer (prev.(RestrFramesDef) cohFrames.1) d -> mkLayer deps.(_restrFrames)
     ((prev.(RestrFramesDef) cohFrames.1).2 q.+1 (⇑ Hq) ε d) :=
-  fun l ω => rew [deps.(_paintings'').2] cohFrames.2 0 q leY_O Hq ε ω d in
-             restrPaintings'.2 q Hq ε _ (l ω).
+  fun l ω => rew [deps.(_paintings).2] cohFrames.2 0 q leY_O Hq ε ω d in
+             restrPaintings.2 q Hq ε _ (l ω).
 
 (** Under previous assumptions, and, additionally:
       [restrPainting(p+n,0);...;restrPainting(p+n,p-1)]
@@ -315,21 +291,21 @@ Definition mkRestrLayer `{deps: DepsRestr p.+1 n}
 #[local]
 Instance mkCohFrameTypesAndRestrFrames:
   forall `{deps: DepsRestr p n} {extraDeps: DepsRestrExtension deps}
-  (restrPaintings': RestrPaintingTypes' extraDeps), CohFrameTypeBlock :=
+  (restrPaintings: RestrPaintingTypes extraDeps), CohFrameTypeBlock :=
   fix mkCohFrameTypesAndRestrFrames {p}:
   forall `(deps: DepsRestr p n) (extraDeps: DepsRestrExtension deps)
-    (restrPaintings': RestrPaintingTypes' extraDeps), CohFrameTypeBlock :=
+    (restrPaintings: RestrPaintingTypes extraDeps), CohFrameTypeBlock :=
   match p with
   | 0 =>
-    fun n deps extraDeps restrPaintings' =>
+    fun n deps extraDeps restrPaintings =>
     {|
       CohFrameTypesDef := unit;
       RestrFramesDef _ := (tt; fun _ _ _ _ => tt)
     |}
   | S p =>
-    fun n deps extraDeps restrPaintings' =>
+    fun n deps extraDeps restrPaintings =>
     let prev := mkCohFrameTypesAndRestrFrames deps.(1)%depsrestr
-      (deps.(2); extraDeps)%extradeps restrPaintings'.1 in
+      (deps.(2); extraDeps)%extradeps restrPaintings.1 in
     let restrFrames := prev.(RestrFramesDef) in
     let cohFrameTypes := prev.(CohFrameTypesDef) in
     {|
@@ -337,9 +313,10 @@ Instance mkCohFrameTypesAndRestrFrames:
       RestrFramesDef Q :=
       (* RestrFrame(n+2,p+1) *)
       let restrFrame q (Hq: q <= n) ε
-        (d: mkFrame (extraDeps := (deps.(2); extraDeps)) (restrFrames Q.1)) :=
+        (d: mkFrame (mkDepsRestr
+          (extraDeps := (deps.(2); extraDeps)) (restrFrames Q.1))) :=
           ((restrFrames Q.1).2 q.+1 (⇑ Hq) ε d.1;
-           mkRestrLayer restrPaintings' Q q _ ε d.1 d.2)
+           mkRestrLayer restrPaintings Q q _ ε d.1 d.2)
       in (restrFrames Q.1; restrFrame)
     |}
   end.
@@ -349,27 +326,27 @@ Instance mkCohFrameTypesAndRestrFrames:
 
 Definition mkCohFrameTypes `{deps: DepsRestr p n}
   {extraDeps: DepsRestrExtension deps}
-  (restrPaintings': RestrPaintingTypes' extraDeps) :=
-  (mkCohFrameTypesAndRestrFrames restrPaintings').(CohFrameTypesDef).
+  (restrPaintings: RestrPaintingTypes extraDeps) :=
+  (mkCohFrameTypesAndRestrFrames restrPaintings).(CohFrameTypesDef).
 
 Class DepsCohs p n := {
   _deps: DepsRestr p n;
   _extraDeps: DepsRestrExtension _deps;
-  _restrPaintings': RestrPaintingTypes' _extraDeps;
-  _cohs: mkCohFrameTypes _restrPaintings';
+  _restrPaintings: RestrPaintingTypes _extraDeps;
+  _cohs: mkCohFrameTypes _restrPaintings;
 }.
 
 #[local]
-Instance mkDepsCohs0 `{deps: DepsRestr p 0} {E': mkFrame' deps -> HSet}
-  {restrPaintings': RestrPaintingTypes' (TopDep E')}
-  (cohs: mkCohFrameTypes restrPaintings'): DepsCohs p 0 := {| _cohs := cohs |}.
+Instance mkDepsCohs0 `{deps: DepsRestr p 0} {E': mkFrame deps -> HSet}
+  {restrPaintings: RestrPaintingTypes (TopDep E')}
+  (cohs: mkCohFrameTypes restrPaintings): DepsCohs p 0 := {| _cohs := cohs |}.
 
 #[local]
 Instance slideDepsCohs `(depsCohs: DepsCohs p.+1 n): DepsCohs p n.+1 :=
 {|
   _deps := depsCohs.(_deps).(1);
   _extraDeps := (depsCohs.(_deps).(2); depsCohs.(_extraDeps));
-  _restrPaintings' := depsCohs.(_restrPaintings').1;
+  _restrPaintings := depsCohs.(_restrPaintings).1;
   _cohs := depsCohs.(_cohs).1;
 |}.
 
@@ -380,7 +357,7 @@ Notation "x .(1)" := (slideDepsCohs x%depscohs)
   (at level 1, left associativity, format "x .(1)"): depscohs_scope.
 
 Definition mkRestrFrames `{depsCohs: DepsCohs p n} :=
-  (mkCohFrameTypesAndRestrFrames depsCohs.(_restrPaintings')).(RestrFramesDef)
+  (mkCohFrameTypesAndRestrFrames depsCohs.(_restrPaintings)).(RestrFramesDef)
     depsCohs.(_cohs).
 
 (* Tying the loop: we type mkRestrFrame((p+1)+n,p) knowing
@@ -391,16 +368,16 @@ Definition mkRestrFrames `{depsCohs: DepsCohs p n} :=
     circular.
     Instead, we only require restrFrames(p+(1+n),0..p-1) then build the type of
     restrFrame(p+1+n,p) as: Frame(p+(1+n),p) -> Frame(p+n,p)
-    At the end, with only the addition of restrPaintings' and cohs, the loop is gone *)
+    At the end, with only the addition of restrPaintings and cohs, the loop is gone *)
 
 Definition mkRestrFrameType `{depsCohs: DepsCohs p n} :=
   forall q (Hq: q <= n) (ε: arity),
-  mkPrevFrame (mkRestrFrames) -> mkFrame' depsCohs.(_deps).
+  mkFrame (mkDepsRestr mkRestrFrames).(1) -> mkFrame depsCohs.(_deps).
 
 Definition mkRestrFrame `{depsCohs: DepsCohs p n}: mkRestrFrameType :=
   mkRestrFrames.2.
 
-(* Example: if p := 0, extraDeps := ([],E'), restrPaintings' := , cohs := []
+(* Example: if p := 0, extraDeps := ([],E'), restrPaintings := , cohs := []
    then mkFullDepsRestr := {_frames'':=[unit];
                        _paintings'':=[E']};
                        _restrFrames':=[\qω().()]}
@@ -410,7 +387,7 @@ Definition mkFullDepsRestr `{depsCohs: DepsCohs p n} :=
   mkDepsRestr mkRestrFrames.
 
 Inductive DepsCohsExtension {p}: forall `(depsCohs: DepsCohs p n), Type :=
-| TopCohFrame `{depsCohs: DepsCohs p 0} (E: mkFrame mkRestrFrames -> HSet):
+| TopCohFrame `{depsCohs: DepsCohs p 0} (E: mkFrame (mkDepsRestr mkRestrFrames) -> HSet):
   DepsCohsExtension depsCohs
 | AddCohFrame {n} (depsCohs: DepsCohs p.+1 n):
   DepsCohsExtension depsCohs -> DepsCohsExtension depsCohs.(1).
@@ -431,26 +408,15 @@ Proof.
     + now exact (mkExtraDeps p.+1 n depsCohs extraDepsCohs).
 Defined.
 
-Definition mkPainting `{depsCohs: DepsCohs p n}
-  (extraDepsCohs: DepsCohsExtension depsCohs):
-  mkFrame mkRestrFrames -> HSet :=
-  mkPainting' (mkExtraDeps extraDepsCohs).
-
-Definition mkPrevPainting `{depsCohs: DepsCohs p n}
-  (extraDepsCohs: DepsCohsExtension depsCohs):
-  mkPrevFrame mkRestrFrames -> HSet :=
-  mkPainting' (mkFullDepsRestr.(2); mkExtraDeps extraDepsCohs)%extradeps.
-
 (* Note: We could type mkRestrPainting(p+1+n,p) of type
    RestrPaintingType(p+1+n,p) up to using unfoldPaintingProj at other places.
-   It is more convenient to refer to mkPrevPainting to later state cohPainting.
 *)
 
 Definition mkRestrPaintingType `{depsCohs: DepsCohs p n}
   (extraDepsCohs: DepsCohsExtension depsCohs) :=
-  forall q (Hq: q <= n) ε (d: mkPrevFrame mkRestrFrames),
-  mkPrevPainting extraDepsCohs d ->
-  (mkPaintings' depsCohs.(_extraDeps)).2 (mkRestrFrame q Hq ε d).
+  forall q (Hq: q <= n) ε (d: mkFrame (mkDepsRestr mkRestrFrames).(1)),
+  mkPainting (mkFullDepsRestr.(2); mkExtraDeps extraDepsCohs)%extradeps d ->
+  (mkPaintings depsCohs.(_extraDeps)).2 (mkRestrFrame q Hq ε d).
 
 (* Note: a priori, unfoldPaintingProj can be avoided because only
    "mkRestrPaintingType 0" and "mkRestrPaintingType p.+1" are later used,
@@ -464,14 +430,14 @@ Proof.
   - destruct extraDepsCohs.
     + exfalso; now apply leY_O_contra in Hq.
     + rewrite <- unfoldPaintingProj. unshelve esplit.
-      * now exact (mkRestrLayer depsCohs.(_restrPaintings') depsCohs.(_cohs)
+      * now exact (mkRestrLayer depsCohs.(_restrPaintings) depsCohs.(_cohs)
         q (⇓ Hq) ε d l).
       * now exact (mkRestrPainting p.+1 n depsCohs extraDepsCohs q (⇓ Hq) ε (d; l) c).
 Defined.
 
 Definition mkRestrPaintingTypes `{depsCohs: DepsCohs p n}
   (extraDepsCohs: DepsCohsExtension depsCohs) :=
-  RestrPaintingTypes' (mkExtraDeps extraDepsCohs).
+  RestrPaintingTypes (mkExtraDeps extraDepsCohs).
 
 Fixpoint mkRestrPaintings `{depsCohs: DepsCohs p n}
   (extraDepsCohs: DepsCohsExtension depsCohs): mkRestrPaintingTypes extraDepsCohs.
@@ -488,13 +454,13 @@ Defined.
 Definition mkCohPaintingType `{depsCohs: DepsCohs p.+1 n}
   (extraDepsCohs: DepsCohsExtension depsCohs) :=
   forall r q (Hrq: r <= q) (Hq: q <= n) (ε ω: arity)
-    (d: mkPrevFrame mkRestrFrames)
-    (c: (mkPaintings' (mkFullDepsRestr.(2);
+    (d: mkFrame (mkDepsRestr mkRestrFrames).(1))
+    (c: (mkPaintings (mkFullDepsRestr.(2);
       mkExtraDeps (depsCohs; extraDepsCohs))).2 d),
-  rew [depsCohs.(_deps).(2).(_painting'')] depsCohs.(_cohs).2 r q Hrq Hq ε ω d in
-  depsCohs.(_restrPaintings').2 q Hq ε _
+  rew [depsCohs.(_deps).(2).(_painting)] depsCohs.(_cohs).2 r q Hrq Hq ε ω d in
+  depsCohs.(_restrPaintings).2 q Hq ε _
     ((mkRestrPaintings (depsCohs; extraDepsCohs)).2 r _ ω d c) =
-  depsCohs.(_restrPaintings').2 r (Hrq ↕ Hq) ω _
+  depsCohs.(_restrPaintings).2 r (Hrq ↕ Hq) ω _
     ((mkRestrPaintings (depsCohs; extraDepsCohs)).2 q.+1 _ ε d c).
 
 Fixpoint mkCohPaintingTypes {p}: forall `{depsCohs: DepsCohs p n}
@@ -507,18 +473,18 @@ Fixpoint mkCohPaintingTypes {p}: forall `{depsCohs: DepsCohs p n}
          mkCohPaintingType extraDepsCohs }
   end.
 
-Lemma mkCoh2Frame `(depsCohs : DepsCohs p.+1 n)
-  (extraDepsCohs : DepsCohsExtension depsCohs)
-  (cohPaintings : mkCohPaintingTypes extraDepsCohs)
-  (prevCohFrames : mkCohFrameTypes
+Lemma mkCoh2Frame `(depsCohs: DepsCohs p.+1 n)
+  (extraDepsCohs: DepsCohsExtension depsCohs)
+  (cohPaintings: mkCohPaintingTypes extraDepsCohs)
+  (prevCohFrames: mkCohFrameTypes
      (extraDeps := (mkFullDepsRestr.(2); mkExtraDeps extraDepsCohs))
      (mkRestrPaintings extraDepsCohs).1) :
-  forall (r q : nat) (Hrq : r <= q) (Hq : q <= n) (ε ω : arity)
-  (d : mkPrevFrame (mkRestrFrames (depsCohs := {| _cohs := prevCohFrames.1 |})))
+  forall (r q: nat) (Hrq: r <= q) (Hq: q <= n) (ε ω: arity)
+  (d : mkFrame (mkDepsRestr (mkRestrFrames (depsCohs := {| _cohs := prevCohFrames.1 |}))).(1))
   (𝛉 : arity),
   f_equal
-    (fun x : mkFrame' depsCohs.(_deps).(1) =>
-     depsCohs.(_deps).(2).(_restrFrame') q ε x)
+    (fun x : mkFrame depsCohs.(_deps).(1) =>
+     depsCohs.(_deps).(2).(_restrFrame) q ε x)
     (prevCohFrames.2 0 r leY_O (Hrq ↕ ↑ Hq) ω 𝛉 d)
   • (depsCohs.(_cohs).2 0 q leY_O Hq ε 𝛉
        (((mkCohFrameTypesAndRestrFrames
@@ -526,22 +492,22 @@ Lemma mkCoh2Frame `(depsCohs : DepsCohs p.+1 n)
          RestrFramesDef) prevCohFrames.1).2 r.+1 (⇑ (Hrq ↕ ↑ Hq)) ω d)
      • f_equal
          (fun x =>
-          depsCohs.(_deps).(_restrFrames').2 0 leY_O 𝛉 x)
+          depsCohs.(_deps).(_restrFrames).2 0 leY_O 𝛉 x)
          (prevCohFrames.2 r.+1 q.+1 (⇑ Hrq) (⇑ Hq) ε ω d)) =
   depsCohs.(_cohs).2 r q Hrq Hq ε ω
     (((mkCohFrameTypesAndRestrFrames
          (mkRestrPaintings (depsCohs;extraDepsCohs)).1).(
       RestrFramesDef) prevCohFrames.1).2 0 leY_O 𝛉 d)
   • (f_equal
-       (fun x : mkFrame' depsCohs.(_deps).(1) =>
-        depsCohs.(_deps).(2).(_restrFrame') r ω x)
+       (fun x : mkFrame depsCohs.(_deps).(1) =>
+        depsCohs.(_deps).(2).(_restrFrame) r ω x)
        (prevCohFrames.2 0 q.+1 leY_O (⇑ Hq) ε 𝛉 d)
      • depsCohs.(_cohs).2 0 r leY_O (Hrq ↕ Hq) ω 𝛉
          (((mkCohFrameTypesAndRestrFrames
               (mkRestrPaintings (depsCohs;extraDepsCohs)).1).(
            RestrFramesDef) prevCohFrames.1).2 q.+2 (⇑ (⇑ Hq)) ε d)).
 Proof.
-  now intros; apply depsCohs.(_deps).(2).(_frame'').(UIP).
+  now intros; apply depsCohs.(_deps).(2).(_frame).(UIP).
 Defined.
 
 Definition mkCohLayer `{depsCohs: DepsCohs p.+1 n}
@@ -551,30 +517,30 @@ Definition mkCohLayer `{depsCohs: DepsCohs p.+1 n}
     (extraDeps := (mkFullDepsRestr.(2); mkExtraDeps extraDepsCohs))
     (mkRestrPaintings extraDepsCohs).1}
   r q {Hrq: r <= q} {Hq: q <= n} (ε ω: arity)
-  (d: mkPrevFrame (mkRestrFrames (depsCohs := {| _cohs := prevCohFrames.1 |})))
+  (d: mkFrame (mkDepsRestr (mkRestrFrames (depsCohs := {| _cohs := prevCohFrames.1 |}))).(1))
   (l: mkLayer mkRestrFrames d):
   rew [mkLayer _] prevCohFrames.2 r.+1 q.+1 (⇑ Hrq) (⇑ Hq) ε ω d in
-    mkRestrLayer depsCohs.(_restrPaintings') depsCohs.(_cohs) q Hq ε _
+    mkRestrLayer depsCohs.(_restrPaintings) depsCohs.(_cohs) q Hq ε _
       (mkRestrLayer (mkRestrPaintings extraDepsCohs).1 _ r (Hrq ↕ ↑ Hq) ω d l) =
-    mkRestrLayer depsCohs.(_restrPaintings') depsCohs.(_cohs) r (Hrq ↕ Hq) ω _
+    mkRestrLayer depsCohs.(_restrPaintings) depsCohs.(_cohs) r (Hrq ↕ Hq) ω _
       (mkRestrLayer (mkRestrPaintings extraDepsCohs).1 _ q.+1 (⇑ Hq) ε d l).
 Proof.
   apply functional_extensionality_dep; intros 𝛉.
   rewrite <- map_subst_app. unfold mkRestrLayer; simpl.
   rewrite
-    <- map_subst with (f := fun x => depsCohs.(_restrPaintings').2 q Hq ε x),
+    <- map_subst with (f := fun x => depsCohs.(_restrPaintings).2 q Hq ε x),
     <- map_subst with
-        (f := fun x => depsCohs.(_restrPaintings').2 r (Hrq ↕ Hq) ω x),
-    -> rew_map with (P := fun x => depsCohs.(_deps).(_paintings'').2 x)
-        (f := fun x => depsCohs.(_deps).(_restrFrames').2 O leY_O 𝛉 x),
-    -> rew_map with (P := fun x => depsCohs.(_deps).(_paintings'').2 x)
-        (f := fun x => depsCohs.(_deps).(2).(_restrFrame') r
+        (f := fun x => depsCohs.(_restrPaintings).2 r (Hrq ↕ Hq) ω x),
+    -> rew_map with (P := fun x => depsCohs.(_deps).(_paintings).2 x)
+        (f := fun x => depsCohs.(_deps).(_restrFrames).2 O leY_O 𝛉 x),
+    -> rew_map with (P := fun x => depsCohs.(_deps).(_paintings).2 x)
+        (f := fun x => depsCohs.(_deps).(2).(_restrFrame) r
           (Hq := Hrq ↕ Hq) ω x),
-    -> rew_map with (P := fun x => depsCohs.(_deps).(_paintings'').2 x)
-        (f := fun x => depsCohs.(_deps).(2).(_restrFrame') q ε x),
+    -> rew_map with (P := fun x => depsCohs.(_deps).(_paintings).2 x)
+        (f := fun x => depsCohs.(_deps).(2).(_restrFrame) q ε x),
     <- cohPaintings.2.
   repeat rewrite rew_compose.
-  apply rew_swap with (P := fun x => depsCohs.(_deps).(_paintings'').2 x).
+  apply rew_swap with (P := fun x => depsCohs.(_deps).(_paintings).2 x).
   rewrite rew_app_rl. now trivial.
   now apply mkCoh2Frame.
 Defined.
@@ -603,16 +569,18 @@ Instance mkDepsCohs `{depsCohs: DepsCohs p n}
 {|
   _deps := mkFullDepsRestr;
   _extraDeps := mkExtraDeps extraDepsCohs;
-  _restrPaintings' := mkRestrPaintings extraDepsCohs;
+  _restrPaintings := mkRestrPaintings extraDepsCohs;
   _cohs := mkCohFrames cohPaintings;
 |}.
 
 Inductive DepsCohs2Extension {p}: forall `{depsCohs: DepsCohs p n}
   {extraDepsCohs: DepsCohsExtension depsCohs},
   mkCohPaintingTypes extraDepsCohs -> Type :=
-| TopCohPainting `{depsCohs: DepsCohs p 0} {E: mkFrame mkRestrFrames -> HSet}
+| TopCohPainting `{depsCohs: DepsCohs p 0}
+  {E: mkFrame (mkDepsRestr mkRestrFrames) -> HSet}
   {cohPaintings: mkCohPaintingTypes (TopCohFrame E)}
-  {NextE: mkFrame (mkRestrFrames (depsCohs := mkDepsCohs cohPaintings)) -> HSet}
+  {NextE: mkFrame
+    (mkDepsRestr (mkRestrFrames (depsCohs := mkDepsCohs cohPaintings))) -> HSet}
   : DepsCohs2Extension cohPaintings
 | AddCohPainting {n} {depsCohs: DepsCohs p.+1 n}
   {extraDepsCohs: DepsCohsExtension depsCohs}
@@ -640,8 +608,8 @@ Defined.
 
 Lemma unfoldRestrPaintings `{depsCohs: DepsCohs p n}
   {extraDepsCohs: DepsCohsExtension depsCohs} q {Hq: q <= n} ε
-  (d: mkFrame' mkFullDepsRestr.(1))
-  (c: (mkPaintings' (mkFullDepsRestr.(2); mkExtraDeps extraDepsCohs)).2 d):
+  (d: mkFrame mkFullDepsRestr.(1))
+  (c: (mkPaintings (mkFullDepsRestr.(2); mkExtraDeps extraDepsCohs)).2 d):
   (mkRestrPaintings extraDepsCohs).2 q Hq ε d c =
   mkRestrPainting extraDepsCohs q Hq ε d (rew <- unfoldPaintingProj in c).
 Proof.
@@ -664,11 +632,11 @@ Proof.
     destruct q. exfalso; now apply leY_O_contra in Hrq.
     destruct extraCohPaintings. exfalso; now apply leY_O_contra in Hq.
     rewrite <- rew_permute_ll_hset with
-      (P := mkPainting' (depsCohs.(_deps).(2); depsCohs.(_extraDeps))).
+      (P := mkPainting (depsCohs.(_deps).(2); depsCohs.(_extraDeps))).
     apply rew_swap.
     do 2 rewrite rew_opp_l.
     unshelve eapply (rew_existT_curried
-      (Q := mkPainting' depsCohs.(_extraDeps))).
+      (Q := mkPainting depsCohs.(_extraDeps))).
     now exact (mkCohLayer cohPaintings r q (Hrq := ⇓ Hrq) ε ω d l).
     now exact (mkCohPainting p.+1 n depsCohs extraDepsCohs
       cohPaintings extraCohPaintings r q (⇓ Hrq) (⇓ Hq) ε ω (d; l) c).
@@ -691,48 +659,46 @@ Defined.
 
 Class νSetAux p := {
   deps: DepsRestr p 0;
-  restrPaintings' E': RestrPaintingTypes' (TopDep E');
-  cohFrames E': mkCohFrameTypes (restrPaintings' E');
+  restrPaintings E': RestrPaintingTypes (TopDep E');
+  cohFrames E': mkCohFrameTypes (restrPaintings E');
   cohPaintings E' E: mkCohPaintingTypes
     (depsCohs := mkDepsCohs0 (cohFrames E')) (TopCohFrame E);
 }.
 
 Class νSet p := {
-  prefix'': Type;
-  data: prefix'' -> νSetAux p;
+  prefix: Type;
+  data: prefix -> νSetAux p;
 }.
 
 (***************************************************)
 (** The construction of [νSet n+1] from [νSet n] *)
 
 (** Extending the initial prefix *)
-Definition mkPrefix'' p {C: νSet p}: Type :=
-  { D: C.(prefix'') &T mkFrame' (C.(data) D).(deps) -> HSet }.
+Definition mkPrefix p {C: νSet p}: Type :=
+  { D: C.(prefix) &T mkFrame (C.(data) D).(deps) -> HSet }.
 
 Section νSetData.
 Variable p: nat.
 Variable C: νSet p.
-Variable D: mkPrefix'' p.
+Variable D: mkPrefix p.
 
-Definition mkDepsCohs'': DepsCohs p 0 :=
+Definition mkDepsCohs': DepsCohs p 0 :=
   mkDepsCohs0 ((C.(data) D.1).(cohFrames) D.2).
 
 Definition mkDepsRestr': DepsRestr p.+1 0 :=
-  mkFullDepsRestr (depsCohs := mkDepsCohs'').
+  mkFullDepsRestr (depsCohs := mkDepsCohs').
 
-Definition mkRestrPaintings' E': RestrPaintingTypes' (TopDep E') :=
-  mkRestrPaintings (depsCohs := mkDepsCohs'') (TopCohFrame E').
+Definition mkRestrPaintings' E': RestrPaintingTypes (TopDep E') :=
+  mkRestrPaintings (depsCohs := mkDepsCohs') (TopCohFrame E').
 
 Definition mkCohFrames' E': mkCohFrameTypes (mkRestrPaintings' E') :=
-  mkCohFrames (depsCohs := mkDepsCohs'')
+  mkCohFrames (depsCohs := mkDepsCohs')
     ((C.(data) D.1).(cohPaintings) D.2 E').
 
-Definition mkDepsCohs' E': DepsCohs p.+1 0 :=
-  mkDepsCohs0 (mkCohFrames' E').
-
 Definition mkCohPaintings' E' E:
-  mkCohPaintingTypes (depsCohs := mkDepsCohs' E') (TopCohFrame E) :=
- mkCohPaintings (TopCohPainting (NextE := E)).
+  mkCohPaintingTypes (depsCohs := mkDepsCohs0 (mkCohFrames' E'))
+    (TopCohFrame E) :=
+  mkCohPaintings (TopCohPainting (NextE := E)).
 
 End νSetData.
 
@@ -746,11 +712,11 @@ Defined.
 #[local]
 Instance mkνSet {p} (C: νSet p): νSet p.+1 :=
 {|
-  prefix'' := mkPrefix'' p;
-  data := fun D: mkPrefix'' p =>
+  prefix := mkPrefix p;
+  data := fun D: mkPrefix p =>
   {|
     deps := mkDepsRestr' p C D;
-    restrPaintings' := mkRestrPaintings' p C D;
+    restrPaintings := mkRestrPaintings' p C D;
     cohFrames := mkCohFrames' p C D;
     cohPaintings := mkCohPaintings' p C D
   |}
@@ -763,8 +729,8 @@ Fixpoint νSetAt n: νSet n :=
   | n.+1 => mkνSet (νSetAt n)
   end.
 
-CoInductive νSetFrom n (X: (νSetAt n).(prefix'')): Type := cons {
-  this: mkFrame' ((νSetAt n).(data) X).(deps) -> HSet;
+CoInductive νSetFrom n (X: (νSetAt n).(prefix)): Type := cons {
+  this: mkFrame ((νSetAt n).(data) X).(deps) -> HSet;
   next: νSetFrom n.+1 (X; this);
 }.
 
@@ -779,5 +745,5 @@ Definition SemiCubical := νSets hbool.
 
 (** Some examples *)
 
-Example SemiSimplicial4 := Eval compute in (νSetAt hunit 4).(prefix'' _).
+Example SemiSimplicial4 := Eval compute in (νSetAt hunit 4).(prefix _).
 Print SemiSimplicial4.
